more SHA256 progress

SHA256/Helpers.v
@@ -200,4 +200,163 @@ Proof.
 Qed.  
 
 
+Definition S1_spec (x : ext_val) : ext_val :=
+  match x with
+  | eseq x => eseq (xor_ev (xor_ev (rotr_ev x 6) (rotr_ev x 11)) (rotr_ev x 25))
+  | _ => eseq nil
+  end.
+
+Lemma S1_eval :
+  forall x,
+    has_type x w32 ->
+    forall GE TE SE,
+      wf_env ge GE TE SE ->
+      forall ex res,
+        eager_eval_expr GE TE SE ex (to_sval x) ->
+        res = (to_sval (S1_spec x)) ->
+        eager_eval_expr GE TE SE (EApp (EVar S1) ex) res.
+Proof.
+  intros.
+  gen_global (33,">>>").
+  gen_global (28,"^").
+  gen_global S1.
+  gen_global (0,"demote").
+  inversion H. subst.
+  e. ag.
+  e. use xor_eval.
+  use xor_eval.
+  use rotr_eval.
+  lv.
+
+  use demote_eval.
+  simpl. f_equal.
+  unfold strictnum. f_equal.
+  unfold strictval_from_bitv.
+  instantiate (1 := (ebit true) :: (ebit true) :: (ebit false) :: nil).
+  reflexivity.
+  unfold ExtToBitvector.to_bitv. simpl.
+  instantiate (2 := 3%nat).
+  simpl. reflexivity. reflexivity. eassumption.
+  solve [repeat econstructor; eauto].
+  use rotr_eval; try lv.
+  use demote_eval.
+  simpl. f_equal.
+  unfold strictnum. f_equal.
+  unfold strictval_from_bitv.
+  instantiate (1 := (ebit true) :: (ebit false) :: (ebit true) :: (ebit true) :: nil).
+  reflexivity.
+  instantiate (2 := 4%nat). reflexivity.
+  reflexivity. eassumption.
+  solve [repeat econstructor; eauto].
+  reflexivity.
+
+  eapply has_type_rotr. eassumption.
+  simpl. unfold Pos.to_nat. simpl. omega.
+  eapply has_type_rotr. eassumption.
+  simpl. unfold Pos.to_nat. simpl. omega.
+
+  use rotr_eval; try lv.
+  use demote_eval.
+  simpl. f_equal.
+  unfold strictnum. f_equal.
+  unfold strictval_from_bitv.
+  instantiate (1 := (ebit true) :: (ebit true) :: (ebit false) :: (ebit false) :: (ebit true) :: nil).
+  reflexivity.
+  unfold ExtToBitvector.to_bitv. simpl.
+  instantiate (2 := 5%nat).
+  reflexivity.
+  reflexivity.
+  eassumption.
+  solve [repeat econstructor; eauto].
+  reflexivity.
+  eapply has_type_xor.
+  eapply has_type_rotr. eassumption.
+  simpl. unfold Pos.to_nat. simpl. omega.
+
+  eapply has_type_rotr. eassumption.
+  simpl. unfold Pos.to_nat. simpl. omega.
   
+  eapply has_type_rotr. eassumption.
+  simpl. unfold Pos.to_nat. simpl. omega.
+Qed.
+
+Definition s0_spec (x : ext_val) : ext_val :=
+  match x with
+  | eseq x => eseq (xor_ev (xor_ev (rotr_ev x 7) (rotr_ev x 18)) (shiftr_ev x 3))
+  | _ => eseq nil
+  end.
+
+Lemma s0_eval :
+  forall x,
+    has_type x w32 ->
+    forall GE TE SE,
+      wf_env ge GE TE SE ->
+      forall ex res,
+        eager_eval_expr GE TE SE ex (to_sval x) ->
+        res = (to_sval (s0_spec x)) ->
+        eager_eval_expr GE TE SE (EApp (EVar s0) ex) res.
+Proof.
+  intros.
+  gen_global (33,">>>").
+  gen_global (31,">>").
+  gen_global (28,"^").
+  gen_global s0.
+  gen_global (0,"demote").
+  inversion H. subst.
+  e. ag.
+  e. use xor_eval.
+  use xor_eval.
+  use rotr_eval.
+  lv.
+
+  use demote_eval.
+  simpl. f_equal.
+  unfold strictnum. f_equal.
+  unfold strictval_from_bitv.
+  instantiate (1 := (ebit true) :: (ebit true) :: (ebit true) :: nil).
+  reflexivity.
+  unfold ExtToBitvector.to_bitv. simpl.
+  instantiate (2 := 3%nat).
+  simpl. reflexivity. reflexivity. eassumption.
+  solve [repeat econstructor; eauto].
+  use rotr_eval; try lv.
+  use demote_eval.
+  simpl. f_equal.
+  unfold strictnum. f_equal.
+  unfold strictval_from_bitv.
+  instantiate (1 := (ebit true) :: (ebit false) :: (ebit false) :: (ebit true) :: (ebit false) :: nil).
+  reflexivity.
+  instantiate (2 := 5%nat). reflexivity.
+  reflexivity. eassumption.
+  solve [repeat econstructor; eauto].
+  reflexivity.
+
+  eapply has_type_rotr. eassumption.
+  simpl. unfold Pos.to_nat. simpl. omega.
+  eapply has_type_rotr. eassumption.
+  simpl. unfold Pos.to_nat. simpl. omega.
+
+  use shiftr_eval; try lv.
+  use demote_eval.
+  simpl. f_equal.
+  unfold strictnum. f_equal.
+  unfold strictval_from_bitv.
+  instantiate (1 := (ebit true) :: (ebit true) :: nil). 
+  reflexivity.
+  unfold ExtToBitvector.to_bitv. simpl.
+  instantiate (2 := 2%nat).
+  reflexivity.
+  reflexivity.
+  eassumption.
+  solve [repeat econstructor; eauto].
+  reflexivity.
+  eapply has_type_xor.
+  eapply has_type_rotr. eassumption.
+  simpl. unfold Pos.to_nat. simpl. omega.
+
+  eapply has_type_rotr. eassumption.
+  simpl. unfold Pos.to_nat. simpl. omega.
+  
+  eapply has_type_shiftr. eassumption.
+  simpl. unfold Pos.to_nat. simpl. omega.
+Qed.
